HeapletwiseLeanSepLog/DecoderStyle.lean
@@ -1,0 +1,47 @@
+import HeapletwiseLeanSepLog.DisjointUnion
+
+abbrev Address := UInt64
+abbrev Byte := UInt8
+abbrev Mem := Std.ExtHashMap Address Byte
+
+structure OnHeapAt
+  {T : Type} (decode : Mem -> Address -> Option T) (addr : Address) : Type
+where
+  val : T
+  mem : Mem
+  connection : decode mem addr = some val
+
+infix:80 " @ " => OnHeapAt /- TODO will this class with @make_implicit_args_explicit ? -/
+
+structure MyRecord where
+  x: UInt64
+  y: UInt64
+
+def myRecord (m : Mem) (a : Address) : Option MyRecord := by sorry
+
+def uint (bitwidth : Nat) (m : Mem) (addr : Address) : Option Nat := by sorry
+
+def array {E : Type} (elem : Mem -> Address -> Option E) (len : Nat) (m : Mem) (a : Address)
+    : Option (List E) :=
+  by sorry /- TODO where to put elem size/offset between elements? Infer using typeclass? -/
+
+def Instr : Type := by sorry
+
+def wp (prog : List Instr) (initial : Mem) (post : Mem -> Prop) : Prop := by sorry
+
+def incFieldX : List Instr := by sorry
+
+theorem incFieldX_correct (a_r : Address) (a_vs : Address)
+  (r : myRecord @ a_r)
+  (vs : (array (uint 8) 16) @ a_vs)
+  (boundX : r.val.x.toNat < UInt64.size - 1)
+  (m : Mem)
+  (D : m.splits [r.mem, vs.mem])
+  (post : Mem -> Prop):
+  (forall r' : myRecord @ a_r,
+    r'.val.x == r.val.x + 1 ->
+    r'.val.y == r.val.y ->
+    m.splits [r'.mem, vs.mem] ->
+    post m) ->
+  wp incFieldX m post
+  := by sorry
