HeapletwiseLeanSepLog/EncoderStyle.lean
@@ -1,0 +1,12 @@
+import HeapletwiseLeanSepLog.DisjointUnion
+
+abbrev Address := UInt64
+abbrev Byte := UInt8
+abbrev Mem := Std.ExtHashMap Address Byte
+
+inductive OnHeapAt
+  {T : Type} (encode : T -> Address -> Option Mem) (addr : Address) : Type
+where
+  | mk (val : T) (mem : Mem) (connection : encode val addr = some mem)
+
+infix:80 " @ " => OnHeapAt /- TODO will this class with @make_implicit_args_explicit ? -/
